mkCohDgnLayer, DgnLayer: progress

theories/νType/νType.v
@@ -635,8 +635,9 @@ Class DgnFrameBlock {n} (C: νType n) p (Prev: DgnFrameBlockPrev C):= {
     C.(FramePrev).(frame') (Hpq ↕ Hq) D -> C.(Frame).(frame) (↓ (Hpq ↕ Hq)) D;
   cohDgnFrame {q r} {Hpr: p.+2 <= r.+2} {Hrq: r.+2 <= q.+2} {Hq: q.+2 <= n} {D}
     (d: C.(FramePrev).(frame'') (Hpr ↕ (Hrq ↕ Hq)) D):
-    dgnFrame (q:=q.+1) (↓ (Hpr ↕ Hrq)) (Hq := Hq) (Prev.(dgnFrame') (q:=r) _ d) =
-    dgnFrame (q:=r) (⇓ Hpr) (Hq := ↓ Hrq ↕ Hq) (Prev.(dgnFrame') (q:=q) (Hpr ↕ Hrq) (Hq:=_) d);
+    dgnFrame (q := q.+1) (↓ (Hpr ↕ Hrq)) (Prev.(dgnFrame') (q := r) _ d) =
+    dgnFrame (q := r) (⇓ Hpr) (Hq := ↓ Hrq ↕ Hq)
+      (Prev.(dgnFrame') (q := q) (Hpr ↕ Hrq) d);
   cohDgnRestrFrame {q r ω} {Hpr: p.+2 <= r.+2} {Hrq: r.+2 <= q.+2}
     {Hq: q.+2 <= n} {D} (d: C.(FramePrev).(frame') (↓ (Hpr ↕ Hrq ↕ Hq)) D):
     (Prev.(dgnFrame') (Hpr ↕ Hrq))
@@ -689,10 +690,10 @@ Class Dgn {n} (C: νType n) := {
   DgnPainting: DgnPaintingBlock C DgnPaintingPrev (@DgnFrame);
 
   DgnLayer {p q} {Hpq: p.+2 <= q.+2} {Hq: q.+2 <= n} {D}
-    (d: C.(FramePrev).(frame') (↓ Hq) D):
-    C.(Layer') d -> C.(Layer) (DgnFrame.(dgnFrame) _ d) :=
+    (d: C.(FramePrev).(frame') (↓ (Hpq ↕ Hq)) D):
+    C.(Layer') d -> C.(Layer) (DgnFrame.(dgnFrame) (⇓ Hpq) d) :=
     fun l ω => rew [C.(PaintingPrev).(painting')]
-    DgnFrame.(cohDgnRestrFrame) d in DgnPaintingPrev.(dgnPainting') _ (l ω);
+    DgnFrame.(cohDgnRestrFrame) d in DgnPaintingPrev.(dgnPainting') Hpq (l ω);
 }.
 
 Arguments DgnFramePrev {n C} _.
@@ -711,11 +712,22 @@ Instance mkDgnFramePrev {n} {G: Dgn (νTypeAt n)}:
 Definition mkDgnLayer {n} {G: Dgn (νTypeAt n)}
   {p q} {Hpq: p.+2 <= q.+2} {Hq: q.+2 <= n.+1}
   {Frame: DgnFrameBlock (νTypeAt n.+1) p mkDgnFramePrev}
-  {D} (d: mkFramePrev.(frame') (↓ (Hpq ↕ Hq)) D):
+  {D} {d: mkFramePrev.(frame') (↓ (Hpq ↕ Hq)) D}:
   mkLayer' (d := d) -> mkLayer (d := Frame.(dgnFrame) (⇓ Hpq) d) :=
   fun l ω => rew [(νTypeAt n).(Painting).(painting) D.2]
     Frame.(cohDgnRestrFrame) d in
     G.(DgnPainting).(dgnPainting) (⇓ Hpq) (l ω).
+
+Definition mkCohDgnLayer {n} {G: Dgn (νTypeAt n)} {p q r}
+  {Hpr: p.+3 <= r.+3} {Hrq: r.+3 <= q.+3} {Hq: q.+3 <= n.+1}
+  {D} {d: mkFramePrev.(frame'') (↓ (Hpr ↕ Hrq ↕ Hq)) D}
+  (l: (νTypeAt n).(Layer') (Hp := ⇓ (Hpr ↕ Hrq ↕ Hq)) d):
+  let sl := mkDgnLayer (Hpq := ⇓ (Hpr ↕ Hrq))
+    (G.(DgnLayer) (Hpq := ⇓ (Hpr ↕ Hrq)) d) in
+  let sl' := mkDgnLayer (Hpq := ⇓ Hpr)
+    (G.(DgnLayer) (Hpq := ↓ (Hpr ↕ Hrq)) d) in
+  rew G.(DgnFrame).(cohDgnRestrFrame) d in
+    sl = sl'.
 
 #[local]
 Instance mkDgnFrame0 {n} {G: Dgn (νTypeAt n)}:
@@ -724,7 +736,7 @@ Instance mkDgnFrame0 {n} {G: Dgn (νTypeAt n)}:
   * intros; now exact tt.
   * now trivial.
   * intros; apply rew_swap with (P := id); now destruct (rew _ in _).
-  * intros. simpl. apply -> (rew_swap _ id). now destruct (rew <- _ in _).
+  * intros; apply rew_swap with (P := id); now destruct (rew <- _ in _).
 Defined.
 
 #[local]
@@ -737,7 +749,10 @@ Instance mkDgnFrameSp {n p} {G: Dgn (νTypeAt n)}
     rewrite (νTypeAt n).(eqFrameSp) in d; destruct d as (d, l).
     now exact (Prev.(dgnFrame) _ d; mkDgnLayer d l).
   * (* cohDgnFrame *)
-    intros. simpl. admit.
+    intros. simpl.
+     (= Frame.(cohDgnFrame) (Hrq := Hrq) d; mkCohDgnLayer l).
+
+    admit.
   * (* cohDgnRestrFrame *)
     intros. simpl. admit.
   * admit.
